src/tls/MITLS.Repr.Finished13.fst
@@ -19,7 +19,7 @@ module MITLS.Repr.Finished13
 (* Summary:
 
    This module encapsulates wire-format representations of
-   Parsers.CertificateVerify13 messages.
+   Parsers.Handshake13.handshake13_m13_finished messges
 
    Its main type, `repr b` is an instance of MITLS.Repr.repr
    instantiated with certificateVerify13_parser
@@ -28,12 +28,13 @@ module LP = LowParse.Low.Base
 module B = LowStar.Monotonic.Buffer
 module HS = FStar.HyperStack
 module R = MITLS.Repr
-module Fin13 = Parsers.Handshake13_m13_finished
 open FStar.Integers
 open FStar.HyperStack.ST
 
-let t = Fin13.handshake13_m13_finished
+module HSM13 = Parsers.Handshake13
+
+let t = HSM13.handshake13_m13_finished
 
 let repr (b:R.slice) =
-  R.repr_p t b Fin13.handshake13_m13_finished_parser
- 
+  R.repr_p t b HSM13.handshake13_m13_finished_parser
+
